Examples/Querying/QueryHooked.v
@@ -23,22 +23,20 @@ Variable deserialize : seq nat -> Data.
 Hypothesis ds_inverse : left_inverse serialize deserialize.
 Definition pq := QueryProtocol qnodes serialize lq.
 
-Variable core_state_to_data : heap -> option Data.
+Variable core_state_to_data : heap -> Data -> Prop.
 
 (* The query hook extracts certain data from the the core protocol *)
 (* local state if it's present there. *)
 Definition query_hook : hook_type :=
-  fun hc hq ms to =>
-    if core_state_to_data hc is Some d
-    then exists rid, ms = rid :: serialize d
-    else True.
+  fun hc hq ms to => 
+    forall d, core_state_to_data hc d -> exists rid, ms = rid :: serialize d.
 
 Definition query_hookz := (1, (plab pc), (plab pq, tresp)) \\-> query_hook.
 
 Definition W : world := ((plab pc \\-> pc) \+ (plab pq \\-> pq), query_hookz).
 
 Hypothesis Lab_neq: lq != (plab pc).
-Hypothesis Nodes_eq: forall d, nodes pc d =i qnodes.
+(* Hypothesis Nodes_eq: forall d, nodes pc d =i qnodes. *)
 
 Lemma W_valid : valid W.
 Proof.
@@ -197,8 +195,8 @@ Hypothesis core_state_stable_step : forall z s data s' n,
   this != z -> network_step (plab pc \\-> pc, Unit) z s s' ->
   n \in qnodes ->
   local_indicator data (getLc s) ->
-  core_state_to_data (getLc' s n) = Some data -> 
-  core_state_to_data (getLc' s' n) = Some data.
+  core_state_to_data (getLc' s n) data  -> 
+  core_state_to_data (getLc' s' n) data.
 
 Lemma prEqC' : (getProtocol (plab pc \\-> pc, Unit) (plab pc)) = pc.
 Proof. by rewrite /getProtocol gen_findPt/=. Qed.
@@ -209,8 +207,8 @@ Lemma core_state_stable_step_W s data s' z :
   network_step W z s s' ->
   z \in qnodes ->
   local_indicator data (getLc s) ->
-  core_state_to_data (getLc' s z) = Some data -> 
-  core_state_to_data (getLc' s' z) = Some data.
+  core_state_to_data (getLc' s z) data -> 
+  core_state_to_data (getLc' s' z) data.
 Proof.
 move=>N H2 G L H1; move:(step_coh H2)=>[C1 C2].
 rewrite eqW' in C1 C2.
@@ -240,8 +238,8 @@ Lemma core_state_stable s data s' z :
   network_rely W this s s' ->
   z \in qnodes ->
   local_indicator data (getLc s) ->
-  core_state_to_data (getLc' s z) = Some data -> 
-  core_state_to_data (getLc' s' z)  = Some data.
+  core_state_to_data (getLc' s z) data -> 
+  core_state_to_data (getLc' s' z) data.
 Proof.
 move=> R Z L. move: (L); rewrite -(@rely_loc' _ _ (plab pc) s s' R)=>L'.
 move: R Z L.
@@ -259,7 +257,7 @@ Qed.
 (* A rely-inductive predicate describing the message story *)
 (***********************************************************)
 Definition msg_story s req_num to data reqs resp :=
-  [/\ core_state_to_data (getLc' s to) = Some data,
+  [/\ core_state_to_data (getLc' s to) data,
      local_indicator data (getLc s) & 
      let: d := getSq s in
      [\/ msg_just_sent d reqs resp req_num to,
@@ -332,13 +330,13 @@ Program Definition read_request_id to :
       [/\ getLq i = qst :-> (reqs, resp),
        local_indicator data (getLc i),
        query_init_state to i &
-       core_state_to_data (getLc' i to) = Some data],
+       core_state_to_data (getLc' i to) data],
    fun (r : nat) m => 
      let: (reqs, resp, data) := rrd in 
      [/\ getLq m = qst :-> (reqs, resp),
        local_indicator data (getLc m),
        query_init_state to m,
-       core_state_to_data (getLc' m to) = Some data &                                              
+       core_state_to_data (getLc' m to) data &                                              
        r = fresh_id reqs]) :=
   Do _ (act (@skip_action_wrapper W this lq pq prEqQ _
                                 (fun s pf => fresh_id (getSt this pf).1))).
@@ -370,14 +368,14 @@ Program Definition send_req_act (rid : nat) (to : nid) :
        local_indicator data (getLc i),
        rid = fresh_id reqs,
        query_init_state to i &
-       core_state_to_data (getLc' i to) = Some data],
+       core_state_to_data (getLc' i to) data],
    fun (r : seq nat) m => 
      let: (reqs, resp, data) := rrd in 
      [/\ getLq m = qst :-> ((to, rid) :: reqs, resp),
       local_indicator data (getLc m),
       r = [:: rid],
       msg_story m rid to data ((to, rid) :: reqs) resp &
-      core_state_to_data (getLc' m to) = Some data])
+      core_state_to_data (getLc' m to) data])
   := Do (send_req rid to).
 
 Next Obligation.
@@ -496,7 +494,7 @@ Definition recv_resp_inv (rid : nat) to
     then [/\ getLq i = qst :-> (reqs, resp),
           local_indicator data (getLc i),
           query_init_state to i,
-          core_state_to_data (getLc' i to) = Some data &
+          core_state_to_data (getLc' i to) data &
           d = data]
     else [/\ getLq i = qst :-> ((to, rid) :: reqs, resp),
           local_indicator data (getLc i) &
@@ -510,14 +508,14 @@ Program Definition receive_resp_loop (rid : nat) to :
     [/\ getLq i = qst :-> ((to, rid) :: reqs, resp),
      local_indicator data (getLc i),
      msg_story i rid to data ((to, rid) :: reqs) resp &
-     core_state_to_data (getLc' i to) = Some data],
+     core_state_to_data (getLc' i to) data],
   fun res m =>
     let: (reqs, resp, data) := rrd in
     exists d, res = Some d /\
      [/\ getLq m = qst :-> (reqs, resp),
       local_indicator data (getLc m),
       query_init_state to m,
-      core_state_to_data (getLc' m to) = Some data &
+      core_state_to_data (getLc' m to) data &
       d = data]) := 
   Do _ (@while this W _ _ recv_resp_cond (recv_resp_inv rid to) _
          (fun _ => Do _ (
@@ -635,14 +633,14 @@ Program Definition request_data_program to :
       [/\ getLq i = qst :-> (reqs, resp),
        local_indicator data (getLc i),
        query_init_state to i &
-       core_state_to_data (getLc' i to) = Some data],
+       core_state_to_data (getLc' i to) data],
     fun res m =>
       let: (reqs, resp, data) := rrd in
       exists d, res = Some d /\
       [/\ getLq m = qst :-> (reqs, resp),
        local_indicator data (getLc m),
        query_init_state to m,
-       core_state_to_data (getLc' m to) = Some data &
+       core_state_to_data (getLc' m to) data &
        d = data]) :=
   Do _ (
      rid <-- read_request_id to;
